aneris/examples/crdt/statelib/proof/stlib_proof.v
@@ -1,0 +1,503 @@
+From stdpp Require Import gmap.
+
+From iris.base_logic Require Import invariants bi.
+From iris.algebra Require Import agree auth excl gmap.
+
+From aneris.algebra Require Import monotone.
+From aneris.aneris_lang
+  Require Import lang network tactics proofmode lifting resources.
+From aneris.aneris_lang.lib
+  Require Import list_proof lock_proof vector_clock_proof serialization_proof
+    map_proof lock_proof network_util_proof inject.
+From aneris.aneris_lang.lib.serialization Require Import serialization_proof.
+From aneris.aneris_lang.lib.vector_clock Require Import vector_clock_proof.
+From aneris.aneris_lang.program_logic Require Import lightweight_atomic.
+From aneris.prelude Require Import misc time.
+
+From aneris.examples.crdt.spec
+  Require Import crdt_events crdt_resources crdt_denot crdt_time crdt_base.
+From aneris.examples.crdt.statelib.resources
+  Require Import resources resources_inv resources_local resources_global resources_lock.
+
+From aneris.examples.crdt.statelib Require Import statelib_code.
+From aneris.examples.crdt.statelib.user_model
+  Require Import params model semi_join_lattices.
+From aneris.examples.crdt.statelib.time Require Import time.
+From aneris.examples.crdt.statelib.STS Require Import utils gst lst mutation.
+From aneris.examples.crdt.statelib.proof
+  Require Import spec events resources utils resources
+    stlib_proof_utils internal_specs.
+
+Instance timeinst : Log_Time := timestamp_time.
+
+
+
+(** Nomenclature:
+  * In this file (in every section) there are physical and logical operations
+  * and states. I will try to use the following names to help reading the proofs
+  * and specifications.
+  *
+  *  → Operations:
+  *    ↪ in AnerisLang      (type: val)  : op_v
+  *    ↪ logical operations (type LogOp) : op_log
+  *
+  *  → States:
+  *    ↪ serialized         (type: val)  : st_serialized
+  *    ↪ in AnerisLang      (type: val)  : st_v
+  *    ↪ logical operations (type LogSt) : st_log
+  *    ↪ local states, STS  (type Lst) : lst
+  *    ↪ global states, STS (type Gst) : lst
+  *
+  * Note on coherence:
+  *
+  * There are coherence predicates over these different versions of operations
+  * and states:
+  *
+  * → Operations:
+  *    ↪ LogOp → val : StLib_Op_Coh
+  *
+  * → States:
+  *    ↪ val   ↔ serialized : StLib_StSerialization
+  *    ↪ LogSt → val        : StLib_St_Coh
+  *    ↪ Lst   → LogSt      : denotation
+  *
+  *)
+
+
+
+Section StateLib_Proof.
+
+  Context `{LogOp: Type, LogSt : Type,
+            !anerisG Mdl Σ, !EqDecision LogOp, !Countable LogOp,
+            !CRDT_Params, !Lattice LogSt, !StLib_Params LogOp LogSt,
+            !Internal_StLibG LogOp Σ, !StLib_GhostNames,
+            st_deser: val, stser: serialization}.
+
+  Notation princ_ev := (@principal (gset (Event LogOp)) cc_subseteq).
+
+  (**       +~~~~~~~~~~~~~~~~~~~~~~~~~~~~~~~+
+            | Specification for [get_state] |
+            +~~~~~~~~~~~~~~~~~~~~~~~~~~~~~~~+       **)
+
+
+  Lemma internal_get_state_spec_holds (i : nat) (saddr : socket_address)
+      (lockv : val) (st_loc : loc) (γ__lock : gname) :
+    {{{ StLib_GlobalInv ∗
+        lock_inv saddr γ__lock lockv i st_loc }}}
+      get_state lockv #st_loc @[ip_of_address saddr]
+    {{{ (getst__fun : val), RET getst__fun; internal_get_state_spec getst__fun i saddr }}}.
+  Proof.
+    iIntros (φ) "[#Hinv #Hislock] Hφ".
+    rewrite/get_state. wp_pures.
+    iApply "Hφ"; clear φ.
+
+    iIntros (Haddr φ) "!> Hpre".
+    wp_pures.
+    wp_apply (acquire_spec with "Hislock").
+    iIntros (v) "(-> & Hlocked & Hlock_aux)".
+    wp_pures.
+    
+    rewrite/lock_inv_aux.
+    iDestruct "Hlock_aux"
+      as (ip phys_st log_st h__own h__for Hip)
+        "(Hloc & %Hcoh & (%f & %Hf & %Hislocal & %isforeign & Hown_loc & Hown_for) & %Hcoh')".
+    rewrite Haddr in Hip.
+    simplify_eq/=.
+    wp_load.
+
+    wp_bind (Lam _ _).
+    wp_apply (aneris_wp_atomic _ _ (↑CRDT_InvName)).
+    iMod "Hpre" as (s1 s2) "[(%f' & %Hf' & %Hlocal & %Hsub & Hown_local & Hown_sub & #Hlocal_snap) Hclose]".
+    wp_pures.
+
+    assert (f = f') as <-; first by apply fin_to_nat_inj.
+    iDestruct (both_agree_agree with "Hown_loc Hown_local")
+      as "(Hown_loc & Hown_local & <-)".
+
+    (* open invariant *)
+    iInv "Hinv" as "> (%g & Hglob_ag & Hglob_snap & %Hv & Hglob_local)" "Hclose'".
+    
+    iDestruct ((forall_fin f) with "Hglob_local")
+      as "[(%S' & [%Hnin Hin] & Hother)
+        (%h__local & %h__foreign & %h__subset &
+          %Hproj & %Hlocal_evs & %Hfor_evs & %Hsub_evs & %Hcc &
+          Hown_local' & Hown_foreign' & Hown_subset' & Hown_cc')]".
+    iDestruct (both_agree_agree with "Hown_sub Hown_subset'")
+      as "(Hown_sub & Hown_subset' & ->)".
+    iDestruct (both_agree_agree with "Hown_for Hown_foreign'")
+      as "(Hown_for & Hown_foreign' & ->)".
+    iDestruct (both_agree_agree with "Hown_local' Hown_loc")
+      as "(Hown_local' & Hown_loc & <-)".
+
+    (** Update. *)
+    iDestruct (
+      (own_update_2 (γ_loc_sub !!! f) _ _ ((1/3 + 2/3)%Qp, to_agree h__foreign))
+      with "Hown_subset' Hown_sub") as ">[Hown_subset' Hown_sub]".
+    { rewrite -pair_op frac_op agree_idemp.
+      assert (1 / 3 + 2 / 3 = 1)%Qp as ->; first compute_done.
+      by apply cmra_update_exclusive. }
+    iDestruct (
+      (own_update (γ_loc_cc !!! f) _
+      (● princ_ev (h__local ∪ h__foreign) ⋅ ◯ princ_ev (h__local ∪ h__foreign)))
+      with "Hown_cc'") as ">[Hown_cc' #Hfrag]";
+      first by apply monotone_update.
+
+    iDestruct ((forall_fin' f) with "[Hown_local' Hown_foreign' Hown_subset' Hown_cc' Hin Hother]") as "Hglob_local".
+    { iSplitL "Hother Hin".
+      - iExists S'. iFrame "%". iFrame "Hother Hin".
+      - iExists h__local, h__foreign, h__foreign.
+        iFrame "%". by iFrame. }
+    iMod ("Hclose'" with "[Hglob_snap Hglob_ag Hglob_local]") as "_".
+    { iNext. iExists g. by iFrame. }
+    iModIntro. wp_pures.
+    iMod ("Hclose" with "[Hown_local Hown_sub]") as "Hφ"; last iModIntro.
+    { repeat iSplit.
+      - iPureIntro.
+        destruct Hcc as [hsub hcc].
+        intros x Hx_in.
+        pose (Hsub _ Hx_in) as Hx_orig.
+        apply (elem_of_union_r _ h__local) in Hx_in as Hx_in'.
+        apply hsub in Hx_in'.
+        apply elem_of_union in Hx_in' as [Hx_in'%Hislocal | Hx_in'];
+          first by exfalso; eauto.
+        exact Hx_in'.
+      - iExists f. iFrame "%". iFrame.
+        iExists f. by iFrame "%".
+      - iFrame "%".
+      - iFrame "%". }
+
+    wp_pures.
+    wp_apply (release_spec with "[$Hislock $Hlocked Hloc Hown_loc Hown_for]").
+    { iExists (ip_of_address saddr), phys_st, log_st, h__local, h__foreign.
+      rewrite Haddr.
+      iFrame "%". iFrame.
+      iSplit; first done.
+      iExists f. by iFrame. }
+
+    iIntros (v) "->". wp_pures.
+    iApply "Hφ".
+  Qed.
+
+
+
+  (**       +~~~~~~~~~~~~~~~~~~~~~~~~~~~+
+            | Speficication of [update] |
+            +~~~~~~~~~~~~~~~~~~~~~~~~~~~+                     **)
+
+  (* TODO: move somewhere else *)
+  Lemma op_coh_sv_val {log_op op} :
+    StLib_Op_Coh log_op op -> ∃ (sv : StLib_SerializableVal), op = StLib_SV_val sv.
+  Proof. Admitted.
+
+  Lemma internal_update_spec_holds (repId : nat) (addr : socket_address)
+      (lockv broadcast__fun mutator__fun : val) (st_loc : loc) (γ__lock : gname) :
+    {{{ StLib_GlobalInv ∗
+        lock_inv addr γ__lock lockv repId st_loc ∗
+        (** TODO: broadcast_spec broadcast__fun i saddr ∗ *)
+        mutator_spec mutator__fun
+    }}}
+      update lockv mutator__fun #repId #st_loc @[ip_of_address addr]
+    {{{ (update__fun : val), RET update__fun; internal_update_spec update__fun repId addr }}}.
+  Proof.
+    iIntros (φ) "(#Hinv & #Hlockinv & #mutatorspec) Hφ".
+    wp_lam. wp_pures.
+    iApply "Hφ". clear φ.
+    iIntros (op_v log_op Haddr_proj Hop_coh).
+    iModIntro. iIntros (φ) "Hpre".
+    wp_pures.
+    wp_apply (acquire_spec with "Hlockinv").
+    iIntros (v) "(-> & Hlocked & HPlock)".
+    pose proof (op_coh_sv_val Hop_coh) as [sv ->].
+    wp_pures.
+    iDestruct "HPlock"
+      as (ip phys_st log_st h__local h__for Hip)
+        "(Hloc & %Hcoh & (%f & %Hf & %Hislocal & %isforeign & Hown_loc & Hown_for) & %Hcoh')".
+    wp_apply (aneris_wp_load with "[Hloc]").
+    { iNext. rewrite Haddr_proj in Hip. by simplify_eq/=. }
+    iIntros "Hloc'".
+    wp_bind (mutator__fun _ _ _).
+    pose (fresh_event (h__local ∪ h__for) log_op repId) as fev.
+    iDestruct ("mutatorspec" $! addr repId phys_st sv (h__local ∪ h__for) fev log_op log_st) as "mutatorspec'".
+    wp_apply aneris_wp_value_fupd.
+    iMod "Hpre" as (h_g h__local' h__sub)
+      "[(Hglobstate &
+      %f' & %Hf' & %Hlocalislocal & %Hsubisforeign & Hown_local' & Hown_sub' & #Hlocsnap)
+      Hother]".
+    assert (f = f') as <-.
+    { apply fin_to_nat_inj. by rewrite Hf Hf'. }
+    iInv "Hinv" as "> (%g & Hglob_ag & Hglob_snap & %Hv & Hglob_local)" "Hclose'".
+    iDestruct ((forall_fin f) with "Hglob_local")
+      as "[(%S & [%Hnin %Hin] & HdefS) (%local & %foreign & %sub & %Hg_proj & %locevs & %forevs & %forevs' & %Hcc & Hloc & Hfor & Hsub & Hcc)]".
+
+    (** Regrouping owned resources to prepare for an update *)
+    Ltac mypairvalid A B :=
+      ( apply pair_valid in A as [_ A]; simpl in A;
+        apply (to_agree_op_inv_L) in A as B; destruct B;
+        rewrite agree_idemp; clear A ).
+    iCombine "Hglob_ag" "Hglobstate" as "Hglobal".
+    iDestruct (own_valid_l with "Hglobal") as "[%Hvalid Hown_global]".
+    mypairvalid Hvalid Hglobal_eq.
+    iCombine "Hown_loc" "Hloc" as "Hown_loc".
+    iDestruct (own_valid_l with "Hown_loc") as "[%Hvalid Hown_local]".
+    mypairvalid Hvalid Hlocal_eq.
+    iCombine "Hown_local" "Hown_local'" as "Hown_local".
+    iDestruct (own_valid_l with "Hown_local") as "[%Hvalid Hown_local]".
+    mypairvalid Hvalid Hlocal_eq.
+    iDestruct (both_agree_agree with "Hown_for Hfor") as "(Hown_for & Hfor & <-)".
+    iDestruct (both_agree_agree with "Hown_sub' Hsub") as "(Hown_sub' & Hsub & <-)".
+
+    assert(1/3 + 2/3 = 1)%Qp as ->; first compute_done.
+    assert(1/3 + 1/3 + 1/3 = 1)%Qp as ->; first compute_done.
+
+    iDestruct (own_update _ _ (((1/3)%Qp, to_agree ( h__local ∪ {[ fev ]} )) ⋅ ((2/3)%Qp, to_agree ( h__local ∪ {[ fev ]} )))
+      with "Hown_local") as "> [Hown_local Hown_local']".
+    { rewrite -pair_op agree_idemp frac_op. by apply cmra_update_exclusive. }
+    iDestruct (own_update _ _ (((1/3)%Qp, to_agree ( g.1 ∪ {[ fev ]} )) ⋅ ((2/3)%Qp, to_agree (g.1 ∪ {[ fev ]} )))
+      with "Hown_global") as "> [Hown_global' Hown_global]".
+    { rewrite -pair_op agree_idemp frac_op. by apply cmra_update_exclusive. }
+    iDestruct (own_update _ _ (● (g.1 ∪ {[ fev ]}))
+      with "Hglob_snap") as "> Hown_global_snap".
+    { rewrite (auth_update_auth g.1 (g.1 ∪ {[fev]})(g.1 ∪ {[fev]})); first done.
+      apply gset_local_update, union_subseteq_l. }
+    iDestruct (own_update _ _ (● princ_ev (h__local ∪ {[ fev ]} ∪ h__sub))
+      with "Hcc") as "> Hcc".
+    { admit. }
+
+    pose (mutator_global_valid g log_op f Hv) as Hv'.
+    assert (fresh_event (g.2 !!! f) log_op f = fev) as Hfev_eq.
+    { unfold fev. by rewrite Hg_proj Hf'. }
+
+    iMod ("Hclose'" with "[HdefS Hfor Hsub Hcc Hown_global' Hown_global_snap Hown_local]") as "_".
+    { iNext.
+      iExists (g.1 ∪ {[ fev ]}, vinsert f (g.2 !!! f ∪ {[ fev ]}) g.2).
+      iFrame "Hown_global' Hown_global_snap".
+      rewrite -Hfev_eq. iFrame "%".
+      iExists (S ∪ {[ f ]}).
+      iSplit.
+      { iPureIntro. intros f'.
+         destruct (decide (f' = f)) as [-> | Hneq%Hin];
+          [ by apply elem_of_union_r, elem_of_singleton
+          | by apply elem_of_union_l ]. }
+      iApply big_sepS_union; first set_solver.
+      iSplitL "HdefS".
+      - admit.
+      - iApply big_sepS_singleton.
+        iExists (h__local ∪ {[ fev ]}), h__for, h__sub.
+        iSplitR.
+        { iPureIntro.
+          rewrite vlookup_insert -Hfev_eq Hg_proj. set_solver. }
+        iSplitR.
+        { iPureIntro.
+          by intros e [He_in%locevs | ->%elem_of_singleton]%elem_of_union. }
+        iSplitR; first by iPureIntro.
+        iSplitR; first by iPureIntro.
+        iSplitR.
+        { iPureIntro. admit. }
+        rewrite Hfev_eq. iFrame. }
+
+    iApply ("mutatorspec'" with "[]").
+    { repeat iSplit; iPureIntro; try done.
+      (** The folliwing admots can be solved by using Hv'. *)
+      - intros Himp.
+        rewrite -Hg_proj in Himp.
+        destruct (fresh_event_not_eq_eid (g.2 !!! f) log_op f (VGst_lhst_valid _ Hv f) fev Himp).
+        by rewrite Hfev_eq.
+      - apply elem_of_union_r, elem_of_singleton. reflexivity.
+      - admit. (** TODO: fresh_event is maximal *)
+      - admit.
+      - admit. (** TODO: fresh_event respects total order *) }
+    assert (Hfev_op: EV_Op fev = log_op); first reflexivity.
+    iDestruct ("Hother"
+      $! fev (g.1 ∪ {[ fev ]}) (h__local ∪ {[ fev ]}) h__for $_)
+      as "Hother".
+    (** TODO: get rid of that modality. 
+    iIntros (st') "[%log_st' [%Hcoh_st' %Hmut]]".
+    wp_bind (_ <- _)%E. wp_store. wp_seq.
+    wp_apply (release_spec with "[$Hlockinv $Hlocked Hloc' Hown_loc Hown_for]").
+    { iExists ip, st', log_st', (h__local ∪ {[ fev ]}), h__for.
+      simplify_eq/=. iFrame "%"; iFrame.
+      rewrite Haddr_proj in Hip.
+      simplify_eq/=. iFrame "%"; iFrame.
+      iSplit.
+      - iExists f. repeat iSplit; try done.
+        + admit.
+        + iFrame. admit. (* oupsi :/ *)
+      - admit. }
+    iIntros (v ->).
+    iApply "Hother".
+    *)
+  Admitted.
+
+
+
+  (**       +~~~~~~~~~~~~~~~~~~~~~~~~~~~~~~+
+            | Speficication of [sendToAll] |
+            +~~~~~~~~~~~~~~~~~~~~~~~~~~~~~~+                  **)
+  Definition internal_sendToAll_spec
+    (h: socket_handle) (sock: socket) (repId: RepId) (sock_addr: socket_address)
+    (dstlist: val) : iProp Σ :=
+    ⌜repId < length CRDT_Addresses⌝ -∗
+    ⌜is_list CRDT_Addresses dstlist⌝ -∗
+    ∀ (m: string), (** TODO: require m to follow the protocol. *)
+    {{{ ⌜ CRDT_Addresses !! repId = Some sock_addr ⌝ ∗
+      ⌜ saddress sock = Some sock_addr ⌝ ∗
+      socket_inv repId h sock_addr sock ∗
+      ∃ (st_v: val) (st_log: LogSt) (h__local h__sub: event_set LogOp),
+        ⌜ s_is_ser StLib_StSerialization st_v m ⌝ ∗
+        ⌜ StLib_St_Coh st_log st_v ⌝ ∗
+        ⌜⟦h__local ∪ h__sub⟧ ⇝ st_log⌝ ∗
+        StLib_OwnLocalSnap repId h__local h__sub }}}
+    sendToAll #(LitSocket h) dstlist #repId $m @[ip_of_address sock_addr]
+    {{{ RET #(); True }}}.
+
+  Lemma internal_sendToAll_spec_holds
+    (h: socket_handle) (sock: socket) (repId: RepId) (sock_addr: socket_address)
+    (dstlist: val) :
+    ⌜repId < length CRDT_Addresses⌝ -∗
+    ⌜is_list CRDT_Addresses dstlist⌝ -∗
+    ∀ (m: string), (** TODO: require m to follow the protocol. *)
+    {{{ socket_inv repId h sock_addr sock ∗
+      ∃ (st_v: val) (st_log: LogSt) (h__local h__sub: event_set LogOp),
+        ⌜ s_is_ser StLib_StSerialization st_v m ⌝ ∗
+        ⌜ StLib_St_Coh st_log st_v ⌝ ∗
+        ⌜⟦h__local ∪ h__sub⟧ ⇝ st_log⌝ ∗
+        StLib_OwnLocalSnap repId h__local h__sub }}}
+    sendToAll #(LitSocket h) dstlist #repId $m @[ip_of_address sock_addr]
+    {{{ RET #(); True }}}.
+  Proof.
+    Ltac myload Hname velim :=
+      (wp_bind(!_)%E;
+      iInv "Hl" as ">(%v' & Hownv & Hloc)" "Hclose";
+      wp_load;
+      iCombine "Hγi" "Hownv" as "H";
+      iDestruct (own_valid_l with "H") as (Hname) "(Hγi & Hownv)";
+      apply pair_valid in Hname as [_ <-%to_agree_op_inv_L];
+      rewrite agree_idemp;
+      iMod ( "Hclose"  with "[Hloc Hownv]") as "_";
+      [ iNext; iExists velim; iFrame "Hownv Hloc" | iModIntro]).
+
+    iIntros (Hi Hislist) "%m !> %φ (#HSocketInv &
+      (%st_v & %sy_log & %h__local & %h__sub & %Hser & %Hdenot & #Hsnap))
+      Hφ".
+    rewrite/sendToAll. do 6 wp_pure _.
+    wp_alloc l as "Hl". wp_let.
+    iMod(own_alloc (1%Qp, to_agree O%nat)) as (γi) "[Hγi Hi]"; first done.
+    iMod (inv_alloc (nroot .@ "jfj") _
+      (∃ (v: nat),
+        own γi ((1/2)%Qp, to_agree v) ∗ l ↦[ip_of_address sock_addr] #v)%I
+        with "[Hi Hl]") as "#Hl".
+    { iNext. iExists O. iFrame "Hi Hl". }
+    iAssert (∃ (v: nat), own γi ((1/2)%Qp, to_agree v))%I with "[Hγi]" as "j";
+      first by iExists O.
+    do 3 wp_pure _. iLöb as "IH".
+    iDestruct "j" as "[%vinit Hγi]".
+    wp_pures.
+    (** Check whether index is valid *)
+    wp_apply (wp_list_length $! Hislist ).
+    iIntros (v) "->".
+    myload Hvalid vinit.
+    wp_pures.
+    destruct (decide (vinit < length CRDT_Addresses)%nat);
+      [rewrite bool_decide_eq_true_2 | rewrite bool_decide_eq_false_2];
+      try lia.
+    - wp_if_true.
+      myload Hvalid vinit. wp_pures.
+      destruct (decide (repId = vinit));
+        [rewrite bool_decide_eq_true_2 | rewrite bool_decide_eq_false_2];
+        try lia.
+      + wp_if_true.
+        myload Hvalid vinit. wp_op.
+        wp_bind (_ <- _)%E.
+        iInv "Hl" as "(%v & Hownv & Hloc)" "Hclose".
+        wp_store.
+        assert (vinit + 1 = S vinit) as ->; first lia.
+        iMod (own_update_2 γi _ _ (1%Qp, to_agree (S vinit)%nat) with "Hownv Hγi")
+          as "[Hγi Hownv]".
+        { rewrite -pair_op frac_op Qp_half_half.
+          by apply cmra_update_exclusive. }
+        iMod ("Hclose" with "[Hloc Hγi]") as "_"; last iModIntro.
+        { iNext. iExists (S vinit). iFrame. }
+        wp_seq.
+        iApply ("IH" with "Hφ"). by iExists (S vinit).
+      + wp_if_false. 
+        myload Hvalis vinit.
+        wp_apply (wp_list_nth_some _ vinit CRDT_Addresses dstlist).
+        { iPureIntro. split; [ assumption | lia ]. }
+        iIntros (elt) "(%r & -> & %Hsome)". apply nth_error_lookup in Hsome.
+        wp_apply wp_unSOME; first by iPureIntro.
+        iIntros "_".
+        wp_pures.
+        wp_bind (SendTo _ _ _)%E.
+        iInv "HSocketInv"
+          as "(%Roup & %Soup &
+            >(Hh & %Hsaddr_eq & %Hsaddr_proj & Hsoup & #Hproto_respected))"
+            "Hclose".
+
+        (** TODO:
+          * require the caller [broadcast] to give those resources away
+          * when calling sendToAll.
+          * (?) difficulty: r is unknown at the call of the function *)
+        wp_apply (aneris_wp_send _  (socket_proto repId) with "[$Hh $Hsoup ]");
+          try done.
+        { admit. }
+        iIntros "[Hh Hsoup]".
+        iMod ("Hclose" with "[$Hh Hsoup]") as "_"; last iModIntro.
+        {  iExists _, _. iFrame "Hsoup". by iFrame "#". }
+        wp_pures.
+        myload Hvalid vinit. wp_op. wp_bind (_ <-  _)%E.
+        iInv "Hl" as "(%v & Hownv & Hloc)" "Hclose".
+        wp_store.
+        assert (vinit + 1 = S vinit) as ->; first lia.
+        iMod (own_update_2 γi _ _ (1%Qp, to_agree (S vinit)%nat) with "Hownv Hγi")
+          as "[Hγi Hownv]".
+        { rewrite -pair_op frac_op Qp_half_half.
+          by apply cmra_update_exclusive. }
+        iMod ("Hclose" with "[Hloc Hγi]") as "_"; last iModIntro.
+        { iNext. iExists (S vinit). iFrame. }
+        wp_seq.
+        iApply ("IH" with "Hφ"). by iExists (S vinit).
+    - wp_if_false.
+      by iApply "Hφ".
+  Admitted.
+
+
+
+  (**       +~~~~~~~~~~~~~~~~~~~~~~~~~~~~~~+
+            | Speficication of [broadcast] |
+            +~~~~~~~~~~~~~~~~~~~~~~~~~~~~~~+                  **)
+(** TODO: Specification of the broadcast function. Inspiration from RCB. **)
+  Definition internal_broadcast_spec
+    (broadcast_fun destlist: val) (repId: RepId) addr h s addr_list : iProp Σ :=
+    ∀ (v: StLib_SerializableVal),
+    ⌜is_list CRDT_Addresses addr_list⌝ -∗
+    ⌜repId < length CRDT_Addresses⌝ -∗
+    ⌜ CRDT_Addresses !! repId = Some addr⌝ -∗
+    ⌜ saddress s = Some addr ⌝ -∗
+    ⌜ sblock s = true ⌝ -∗
+    addr ⤇ (socket_proto repId) -∗
+    socket_inv repId h addr s -∗
+    <<< ∀∀ (h__global h__local h__for : event_set LogOp),
+      StLib_OwnGlobalSnap h__global ∗
+      StLib_OwnLocalState repId h__local h__for >>>
+      broadcast_fun #() @[ip_of_address addr] ↑CRDT_InvName
+    <<<▷  RET #(); False >>>.
+
+  (** WIP *)
+
+
+
+  (**       +~~~~~~~~~~~~~~~~~~~~~~~~~~~~~~~~~+
+            | Speficication of [apply_thread] |
+            +~~~~~~~~~~~~~~~~~~~~~~~~~~~~~~~~~+               **)
+  (** WIP *)
+
+
+
+  (**       +~~~~~~~~~~~~~~~~~~~~~~~~~~~~~~~~~~+
+            | Speficication of [statelib_init] |
+            +~~~~~~~~~~~~~~~~~~~~~~~~~~~~~~~~~~+              **)
+  (** Not proven yet. *)
+
+
+End StateLib_Proof.
+
